atoi spec proof + modifications to original functions

Proofs/Helpers/SpecificationProof.v
@@ -1,16 +1,15 @@
-Require Import Utf8.
-Require Import NArith.
 Require Import ZArith.
 Require Import Lia.
 
 Require Import Whitespace.
 Require Import Sign.
 Require Import Digits.
-Require Import BitWidth.
 Require Import Specification.
-Require Import Invariants.
 
-(* ===prove that whitespace works=== *) 
+Require Import Picinae_armv8_pcode.
+Import ARM8Notations.
+
+(* === prove that whitespace works === *) 
 Close Scope Z.
 Theorem whitespace_handler_correct: 
 forall (mem:memory) (p:addr) (w:nat), 
@@ -18,20 +17,20 @@ forall (mem:memory) (p:addr) (w:nat),
   
 Proof. 
   intros. revert p. induction w.
-    intros. simpl. Search (_+0). rewrite N.add_0_r. split; apply N.le_refl.
+    intros. simpl. rewrite N.add_0_r. split; apply N.le_refl.
     intros. simpl. specialize (IHw (p+1)). split; lia.
 Qed.
 
-(* ===prove that sign handling works=== *) 
-(* the sign pointer moves correctly, moves AT MOST one space *) 
+(* === prove that sign handling works === *) 
+(* the pointer doesnt move if theres no sign *) 
 Theorem sign_point_no_sign:
   forall (mem:memory) (p:addr),
-    (Z.of_N (mem \u24b7[ p ]) <> Z.of_N 43) /\
-    (Z.of_N (mem \u24b7[ p ]) <> Z.of_N 45)
+    (Z.of_N (mem Ⓑ[ p ]) <> Z.of_N 43) /\
+    (Z.of_N (mem Ⓑ[ p ]) <> Z.of_N 45)
     -> handle_sign_space mem p = p.
 Proof. 
   intros. unfold handle_sign_space. destruct H as [H43 H45]. 
-  set (x := Z.of_N (mem \u24b7[p])).
+  set (x := Z.of_N (mem Ⓑ[p])).
     destruct (Z.eq_dec x 45) as [Hx45 | Hx45].
       exfalso. apply H45. assumption.
     destruct (Z.eq_dec x 43) as [Hx43 | Hx43].
@@ -39,19 +38,19 @@ Proof.
     reflexivity.
 Qed.
 
-(*  *)
+(* the pointer moves one space if theres a sign *)
 Theorem sign_point_has_sign:
   forall (mem:memory) (p:addr),
-    (Z.of_N (mem \u24b7[ p ]) = Z.of_N 43) \/
-    (Z.of_N (mem \u24b7[ p ]) = Z.of_N 45)
+    (Z.of_N (mem Ⓑ[ p ]) = Z.of_N 43) \/
+    (Z.of_N (mem Ⓑ[ p ]) = Z.of_N 45)
     -> handle_sign_space mem p = p+1.
 Proof.
   intros. unfold handle_sign_space.
-  set (x := Z.of_N (mem \u24b7[p])).
+  set (x := Z.of_N (mem Ⓑ[p])).
     destruct H as [Hx43 | Hx45].
     (* x = 43 *) 
       destruct (Z.eq_dec x 45).
-      simpl. reflexivity.    (* 43 \u2260 45 *)
+      simpl. reflexivity.    
       destruct (Z.eq_dec x 43).
         simpl. reflexivity.
         contradiction.
@@ -67,35 +66,28 @@ Theorem sign_value_correct:
   forall (mem:memory) (p:addr), 
     handle_sign mem p = 1 \/ handle_sign mem p = -1.
 Proof. 
-  intros. unfold handle_sign. destruct (Z.eq_dec (Z.of_N (mem \u24b7[ p ])) 45); auto.
+  intros. unfold handle_sign. destruct (Z.eq_dec (Z.of_N (mem Ⓑ[ p ])) 45); auto.
 Qed.
-
-(*
-  Definition handle_sign (mem:memory) (p:addr) :=
-  let x := Z.of_N(mem \u24b7[p]) in
-  if (Z.eq_dec x 45) then -1
-  else 1.
-*)
 
 Theorem sign_value_neg:
   forall (mem:memory) (p:addr),
-    (Z.of_N (mem \u24b7[ p ]) = Z.of_N 45) -> handle_sign mem p = -1.
+    (Z.of_N (mem Ⓑ[ p ]) = Z.of_N 45) -> handle_sign mem p = -1.
 Proof.
-  intros. unfold handle_sign. destruct (Z.eq_dec (Z.of_N (mem \u24b7[ p ])) 45).
+  intros. unfold handle_sign. destruct (Z.eq_dec (Z.of_N (mem Ⓑ[ p ])) 45).
     reflexivity. contradiction.
 Qed.
 
-
+(* positive sign value *)
 Theorem sign_value_pos:
   forall (mem:memory) (p:addr),
-    (Z.of_N (mem \u24b7[ p ]) <> Z.of_N 45) -> handle_sign mem p = 1.
+    (Z.of_N (mem Ⓑ[ p ]) <> Z.of_N 45) -> handle_sign mem p = 1.
 Proof.
-  intros. unfold handle_sign. destruct (Z.eq_dec (Z.of_N (mem \u24b7[ p ])) 45).
+  intros. unfold handle_sign. destruct (Z.eq_dec (Z.of_N (mem Ⓑ[ p ])) 45).
   contradiction. reflexivity.  
 Qed.
 
 
-(* prove that digits read properly *) 
+(* === prove that digits read properly === *) 
 (* returns some number *) 
 Theorem digit_handler_correct: 
   forall (mem:memory) (p:addr) (k:nat), 
@@ -104,8 +96,8 @@ Proof.
   intros. induction k; lia.
 Qed.
 
-(* prove that parser works *) 
-(*  *)
+(* === prove that parser works === *) 
+(* our number is either 0, a positive, or a negative *)
 Theorem atoi_sign_correct :
   forall mem p w d,
     let z := atoi mem p w d in
@@ -121,15 +113,12 @@ Proof.
   unfold atoi.
   set (p_ws := handle_whitespace mem p w).
   set (p_start := handle_sign_space mem p_ws).
-
-  destruct (handle_digits mem p_start d 0) as [| val].
-    (* handle_digits = 0 *)
-    left. reflexivity.
-    (* handle_digits = S val *)
-    right.
-    set (z := handle_sign mem p_ws).
-
-    (* split on sign *)
+    destruct (handle_digits mem p_start d 0) as [| val].
+      (* handle_digits = 0 *)
+      left. reflexivity.
+      (* handle_digits = S val *)
+      right.
+      set (z := handle_sign mem p_ws).
     destruct (Z.eq_dec z 1); try lia.
       right.
       assert (z = -1).
